examples/knot/Knot1.v
@@ -8,16 +8,12 @@ Require Import PCM.
 Require Import HoareDef.
 Require Import TODOYJ.
 Require Import Logic.
+Require Import KnotHeader.
 
 Generalizable Variables E R A B C X Y Σ.
 
 Set Implicit Arguments.
 
-
-
-Definition knotRA: URA.t := Auth.t (Excl.t (nat -> nat)).
-Definition knot_full (f: option (nat -> nat)) : (@URA.car knotRA) := Auth.black (M:=(Excl.t _)) f.
-Definition knot_frag (f: option (nat -> nat)) : (@URA.car knotRA) := Auth.white (M:=(Excl.t _)) f.
 
 
 
@@ -33,33 +29,16 @@ Section KNOT.
   Section SKENV.
     Variable skenv: SkEnv.t.
 
-    Definition rec_spec:    fspec := mk_simple "Knot" (X:=(nat -> nat) * nat)
-                                               (fun '(f, n) => (
-                                                    (fun varg o => Own (GRA.embed (knot_frag (Some f))) ** ⌜varg = [Vint (Z.of_nat n)]↑ /\ o = ord_pure (2 * n - 1)⌝),
-                                                    (fun vret => ⌜vret = (Vint (Z.of_nat (f n)))↑⌝)
-                                               )).
-
     Definition KnotRecStb: list (gname * fspec) := [("rec", rec_spec)].
 
-    Definition fun_gen (f: nat -> nat) (mn: mname): fspec :=
-      mk_simple mn (X:=nat)
-                (fun n => (
-                     (fun varg o =>
-                        ⌜exists fb fn,
-                            varg = [Vptr fb 0; Vint (Z.of_nat n)]↑ /\ o = ord_pure (2 * n) /\
-                            skenv.(SkEnv.blk2id) fb = Some fn /\
-                            List.find (fun '(_fn, _) => dec fn _fn) (RecStb skenv) = Some (fn, rec_spec)⌝ ** Own (GRA.embed (knot_frag (Some f)))),
-                     (fun vret => ⌜vret = (Vint (Z.of_nat (f n)))↑⌝)
-                )).
-
     Definition knot_spec:    fspec :=
-      mk_simple "Knot" (X:=(nat -> nat))
+      mk_simple (X:=(nat -> nat))
                 (fun f => (
                      (fun varg o =>
                         ⌜exists fn fb,
                             varg = [Vptr fb 0]↑ /\ o = ord_pure 0 /\
                             skenv.(SkEnv.blk2id) fb = Some fn /\
-                            List.find (fun '(_fn, _) => dec fn _fn) (FunStb skenv) = Some (fn, fun_gen f fn)⌝ ** Exists old, Own (GRA.embed (knot_frag old))),
+                            List.find (fun '(_fn, _) => dec fn _fn) (FunStb skenv) = Some (fn, fun_gen RecStb skenv f)⌝ ** Exists old, Own (GRA.embed (knot_frag old))),
                      (fun vret => ⌜exists fn fb,
                             vret = (Vptr fb 0)↑ /\
                             skenv.(SkEnv.blk2id) fb = Some fn /\
@@ -71,19 +50,21 @@ Section KNOT.
     Definition KnotSbtb: list (gname * fspecbody) :=[("rec", mk_specbody rec_spec (fun _ => trigger (Choose _)));
                                                     ("knot", mk_specbody knot_spec (fun _ => trigger (Choose _)))].
 
-    Definition KnotSem: ModSem.t := {|
-      ModSem.fnsems := List.map (fun '(fn, body) => (fn, fun_to_tgt (GlobalStb skenv) fn body)) KnotSbtb;
-      ModSem.mn := "Knot";
-      ModSem.initial_mr := ε;
-      ModSem.initial_st := tt↑;
+    Definition SKnotSem: SModSem.t := {|
+      SModSem.fnsems := KnotSbtb;
+      SModSem.mn := "Knot";
+      SModSem.initial_mr := GRA.embed (knot_full None);
+      SModSem.initial_st := tt↑;
     |}
     .
   End SKENV.
 
-  Definition Knot: Mod.t := {|
-    Mod.get_modsem := fun skenv => KnotSem skenv;
-    Mod.sk := [("rec", Sk.Gfun)];
+  Definition SKnot: SMod.t := {|
+    SMod.get_modsem := SKnotSem;
+    SMod.sk := [("rec", Sk.Gfun)];
   |}
   .
+
+  Definition Knot: Mod.t := (SMod.to_tgt GlobalStb) SKnot.
 
 End KNOT.
