examples/knot/Knot01proof.v
@@ -1,4 +1,4 @@
-Require Import HoareDef Knot0 Knot1 SimModSemL SimModSem.
+Require Import HoareDef KnotHeader Knot0 Knot1 SimModSemL SimModSem.
 Require Import Coqlib.
 Require Import Universe.
 Require Import Skeleton.
@@ -27,6 +27,30 @@ Local Open Scope nat_scope.
 
 
 
+
+(* copied from BW01proof *)
+Section AUX.
+  Context `{Σ: GRA.t}.
+  Context `{@GRA.inG knotRA Σ}.
+  Lemma knot_ra_merge
+        f0 f1
+    :
+      iHyp (Own (GRA.embed (knot_full f0)) -* Own (GRA.embed (knot_frag f1)) -* (⌜f1 = f0⌝)) ε
+  .
+  Proof.
+    iIntro. iIntro.
+    {
+      iMerge A A0. rewrite <- own_sep in A. rewrite GRA.embed_add in A.
+      iOwnWf A. eapply GRA.embed_wf in WF. des. eapply Auth.auth_included in WF. des.
+      eapply Excl.extends in WF; ss.
+      - des; clarify.
+      - ur; ss.
+    }
+  Qed.
+
+End AUX.
+
+
 Section SIMMODSEM.
 
   Context `{Σ: GRA.t}.
@@ -34,24 +58,22 @@ Section SIMMODSEM.
 
   Let W: Type := (Σ * Any.t) * (Σ * Any.t).
 
-  Let wf: W -> Prop :=
-    fun '(mrps_src0, mrps_tgt0) =>
-      exists (mr: Σ) (f: option (nat -> nat)),
-        (<<SRC: mrps_src0 = (mr, tt↑)>>) /\
-        (<<TGT: mrps_tgt0 = (ε, f↑)>>) /\
-        (<<SIM: (iHyp (Own (GRA.embed (bw_full (Z.odd n)))) mr)>>)
-  .
-
-
-  Let wf: W -> Prop :=
-    fun '(mrps_src0, mrps_tgt0) =>
-      (<<SRC: mrps_src0 = (ε, tt↑)>>) /\
-      (<<TGT: mrps_tgt0 = (ε, tt↑)>>)
-  .
-
   Variable RecStb: SkEnv.t -> list (gname * fspec).
   Variable FunStb: SkEnv.t -> list (gname * fspec).
   Variable GlobalStb: SkEnv.t -> list (gname * fspec).
+
+  Let wf (skenv: SkEnv.t): W -> Prop :=
+    fun '(mrps_src0, mrps_tgt0) =>
+      exists (mr: Σ) (f': option (nat -> nat)) (fb': option block),
+        (<<SRC: mrps_src0 = (mr, tt↑)>>) /\
+        (<<TGT: mrps_tgt0 = (ε, fb'↑)>>) /\
+        (<<SIM: (iHyp (Own (GRA.embed (knot_full f'))) mr)>>) /\
+        (<<SOME: forall f (FUN: f' = Some f),
+            exists fb fn,
+              (<<BLK: fb' = Some fb>>) /\
+              (<<FN: skenv.(SkEnv.blk2id) fb = Some fn>>) /\
+              (<<FIND: List.find (fun '(_fn, _) => dec fn _fn) (FunStb skenv) = Some (fn, fun_gen RecStb skenv f)>>)>>)
+  .
 
   Variable RecStb_incl
     :
@@ -69,30 +91,68 @@ Section SIMMODSEM.
   Proof.
     econs; ss; [|admit ""].
     i. eapply adequacy_lift.
-    econstructor 1 with (wf:=wf); et; ss.
-    econs; ss. init. unfold wrapF, ccall. harg_tac.
-    destruct x as [[n0 n1] f]. ss. des; subst.
-    iPure PRE. des; clarify.
-    eapply Any.upcast_inj in PRE. des; clarify.
-    rewrite Any.upcast_downcast. ss. steps. astart 1.
-    rewrite PRE1. ss. steps. rename fn into fn0.
-    hexploit CmpsStb_incl; eauto. i. des.
-    eapply APC_step_clo with (fn:=fn0) (args:=[Vint n0; Vint n1]).
-    { try by
-      eapply Ord.eq_lt_lt;
-       [ symmetry; eapply OrdArith.add_from_nat
-       | eapply OrdArith.lt_from_nat; eapply Nat.lt_add_lt_sub_r;
-          eapply Nat.lt_succ_diag_r ]. }
-    { eauto. }
-    { ss. }
-    { eapply OrdArith.lt_from_nat; eapply Nat.lt_succ_diag_r. }
-    i. subst args'.
-    hcall_tac (n0, n1) (ord_pure 0) (@URA.unit Σ) (@URA.unit Σ) (@URA.unit Σ); ss.
-    { splits; ss. eauto with ord_step. }
-    des. iPure POST. clarify. eapply Any.upcast_inj in POST. des; clarify.
-    steps. rewrite Any.upcast_downcast in _UNWRAPN. clarify. astop.
-    force_l. eexists.
-    hret_tac (@URA.unit Σ) (@URA.unit Σ); ss.
+    econstructor 1 with (wf:=wf skenv); et; ss.
+    2: { eexists. exists None. esplits; ss. eexists. eapply URA.unit_id. }
+    econs; ss; [|econs; ss].
+    { init. unfold recF, ccall. harg_tac.
+      destruct x as [f n]. ss. des. subst.
+      iRefresh. iDestruct PRE. iPure A. des; clarify.
+      eapply Any.upcast_inj in A. des; clarify. steps.
+      rewrite Any.upcast_downcast in _UNWRAPN. clarify. astart 1.
+      assert (f' = Some f); subst.
+      { hexploit knot_ra_merge; et. intro T. iSpecialize T SIM. iSpecialize T PRE. iPure T. auto. }
+      hexploit SOME; eauto. clear SOME. i. des. clarify. steps.
+      rewrite Any.upcast_downcast. ss. steps. rewrite FN. ss. steps.
+      hexploit (SKINCL "rec"); ss; eauto. i. des. rewrite H0. ss. steps.
+      eapply APC_step_clo with (fn0:=fn) (args:=[Vptr blk 0; Vint (Z.of_nat n)]).
+      { try by
+            eapply Ord.eq_lt_lt;
+          [ symmetry; eapply OrdArith.add_from_nat
+          | eapply OrdArith.lt_from_nat; eapply Nat.lt_add_lt_sub_r;
+            eapply Nat.lt_succ_diag_r ]. }
+      { eauto. }
+      { ss. }
+      { eapply OrdArith.lt_from_nat; eapply Nat.lt_succ_diag_r. }
+      i. subst args'. iRefresh.
+      hcall_tac n (ord_pure (2 * n)) SIM (@URA.unit Σ) PRE; ss.
+      { splits; ss. iRefresh. iSplitR PRE; ss.
+        red. red. esplits; eauto.
+        { eapply SKWF. eauto. }
+        { eapply RecStb_incl. des_ifs. }
+      }
+      { splits; ss. eauto with ord_step. }
+      { esplits; eauto. i. clarify. esplits; eauto. }
+      des. clarify. iRefresh. iDestruct POST. iPure POST.
+      eapply Any.upcast_inj in POST. des; clarify.
+      steps. rewrite Any.upcast_downcast in _UNWRAPN. clarify.
+      astop. force_l. eexists.
+      hret_tac SIM0 A; ss.
+      { split; ss. iRefresh. iSplitL A; ss. }
+      { esplits; eauto. }
+    }
+    { init. unfold knotF, ccall. harg_tac.
+      ss. des. subst.
+      iRefresh. iDestruct PRE. iPure PRE. des; clarify.
+      iDestruct A. eapply Any.upcast_inj in PRE. des; clarify. steps.
+      rewrite Any.upcast_downcast in _UNWRAPN. clarify. astart 0. astop.
+      steps. hexploit (SKINCL "rec"); ss; eauto. i. des. rewrite H0. ss. steps.
+      iRefresh. iMerge SIM A.
+
+      rewrite <- own_sep in SIM.
+      eapply own_upd in SIM; cycle 1; [|rewrite intro_iHyp in SIM;iUpdate SIM].
+      { rewrite GRA.embed_add. eapply GRA.embed_updatable.
+        instantiate (1:= knot_full (Some x) ⋅ knot_frag (Some x)).
+        eapply Auth.auth_update. rr. ii. des; ss. ur in FRAME. ur. destruct ctx; ss; clarify.
+      }
+      rewrite <- GRA.embed_add in SIM. rewrite own_sep in SIM. iDestruct SIM.
+      force_l. eexists.
+      hret_tac SIM A; ss.
+      { esplits; eauto. iRefresh. iSplitR A; eauto. red. red. esplits; eauto.
+        { eapply SKWF; eauto. }
+        { eapply RecStb_incl; eauto. }
+      }
+      { esplits; eauto. i. clarify. esplits; eauto. }
+    }
   Qed.
 
 End SIMMODSEM.
