examples/knot/KnotMain01proof.v
@@ -1,0 +1,185 @@
+Require Import HoareDef KnotHeader KnotMain0 KnotMain1 Knot1 SimModSemL SimModSem.
+Require Import Coqlib.
+Require Import Universe.
+Require Import Skeleton.
+Require Import PCM.
+Require Import ModSem Behavior.
+Require Import Relation_Definitions.
+
+(*** TODO: export these in Coqlib or Universe ***)
+Require Import Relation_Operators.
+Require Import RelationPairs.
+From ITree Require Import
+     Events.MapDefault.
+From ExtLib Require Import
+     Core.RelDec
+     Structures.Maps
+     Data.Map.FMapAList.
+
+Require Import HTactics Logic YPM TODOYJ.
+
+Generalizable Variables E R A B C X Y.
+
+Set Implicit Arguments.
+
+Local Open Scope nat_scope.
+
+
+
+
+
+
+Section SIMMODSEM.
+
+  Context `{Σ: GRA.t}.
+  Context `{@GRA.inG knotRA Σ}.
+
+  Let W: Type := (Σ * Any.t) * (Σ * Any.t).
+
+  Variable RecStb: SkEnv.t -> list (gname * fspec).
+  Variable FunStb: SkEnv.t -> list (gname * fspec).
+  Variable GlobalStb: SkEnv.t -> list (gname * fspec).
+
+  Let wf: W -> Prop :=
+    fun '(mrps_src0, mrps_tgt0) =>
+      (<<SRC: mrps_src0 = (ε, tt↑)>>) /\
+      (<<TGT: mrps_tgt0 = (ε, tt↑)>>)
+  .
+
+  Variable RecStb_incl
+    :
+      forall skenv fn fsp
+             (SPECS: List.find (fun '(_fn, _) => dec fn _fn) (RecStb skenv) = Some fsp),
+        List.find (fun '(_fn, _) => dec fn _fn) (GlobalStb skenv) = Some fsp.
+
+  Variable FunStb_incl
+    :
+      forall skenv fn fsp
+             (SPECS: List.find (fun '(_fn, _) => dec fn _fn) (MainFunStb RecStb skenv) = Some fsp),
+        List.find (fun '(_fn, _) => dec fn _fn) (FunStb skenv) = Some fsp.
+
+  Hypotheses GlobalStb_knot
+    :
+      forall skenv,
+        List.find (fun '(_fn, _) => dec "knot" _fn) (GlobalStb skenv) = Some ("knot", knot_spec RecStb FunStb skenv).
+
+  Theorem correct: ModPair.sim (KnotMain1.Main RecStb GlobalStb) KnotMain0.Main.
+  Proof.
+    econs; ss; [|admit ""].
+    i. eapply adequacy_lift.
+    econstructor 1 with (wf:=wf); et; ss.
+    econs; ss; [|econs; ss].
+    { init. unfold fibF, ccall. harg_tac.
+      ss. des. subst.
+      iRefresh. iDestruct PRE. iPure PRE. des; clarify.
+      eapply Any.upcast_inj in PRE. des; clarify. steps.
+      rewrite Any.upcast_downcast in _UNWRAPN. clarify. astart 2. steps.
+      rewrite PRE1. ss. steps.
+      des_ifs.
+      { astop. steps. force_l. eexists.
+        hret_tac (@URA.unit Σ) A; ss. esplits; eauto.
+        iRefresh. iSplitR A; ss. red. red. f_equal. f_equal.
+        clear - l. destruct x; ss. destruct x; ss. lia.
+      }
+      steps.
+      eapply APC_step_clo with (fn0:=fn) (args:=[Vint (Z.of_nat x - 1)]).
+      { try by
+            eapply Ord.eq_lt_lt;
+          [ symmetry; eapply OrdArith.add_from_nat
+          | eapply OrdArith.lt_from_nat; eapply Nat.lt_add_lt_sub_r;
+            eapply Nat.lt_succ_diag_r ]. }
+      { eauto. }
+      { ss. }
+      { eapply OrdArith.lt_from_nat; eapply Nat.lt_succ_diag_r. }
+      i. subst args'. iRefresh.
+      hcall_tac (Fib, x - 1) (ord_pure (2 * x - 1)) (@URA.unit Σ) (@URA.unit Σ) A; ss.
+      { splits; ss. iRefresh. iSplitL A; ss.
+        red. red. esplits; eauto.
+        { repeat f_equal. clear - g. lia. }
+        { f_equal. clear - g. eauto with ord_step. }
+      }
+      { esplits; ss. eauto with ord_step. }
+      steps. des. clarify. iRefresh. iDestruct POST. iPure A.
+      rewrite Any.upcast_downcast in _UNWRAPN. clarify.
+      eapply Any.upcast_inj in A. des; clarify. steps.
+      eapply APC_step_clo with (fn0:=fn) (args:=[Vint (Z.of_nat x - 2)]).
+      { try by
+            eapply Ord.eq_lt_lt;
+          [ symmetry; eapply OrdArith.add_from_nat
+          | eapply OrdArith.lt_from_nat; eapply Nat.lt_add_lt_sub_r;
+            eapply Nat.lt_succ_diag_r ]. }
+      { eauto. }
+      { ss. }
+      { eapply OrdArith.lt_from_nat; eapply Nat.lt_succ_diag_r. }
+      i. subst args'. iRefresh.
+      hcall_tac (Fib, x - 2) (ord_pure (2 * (x - 1) - 1)) (@URA.unit Σ) (@URA.unit Σ) POST; ss.
+      { splits; ss. iRefresh. iSplitL POST; ss.
+        red. red. esplits; eauto.
+        { repeat f_equal. clear - g. lia. }
+        { f_equal. clear - g. eauto with ord_step. }
+      }
+      { esplits; ss. eauto with ord_step. }
+      steps. des. clarify. iRefresh. iDestruct POST0. iPure A.
+      rewrite Any.upcast_downcast in _UNWRAPN. clarify.
+      eapply Any.upcast_inj in A. des; clarify. steps.
+      astop. force_l. eexists.
+      hret_tac (@URA.unit Σ) POST0; ss.
+      splits; ss. iRefresh. iSplitR POST0; ss. red. red.
+      repeat f_equal. destruct x; ss. destruct x; ss.
+      clear - g.
+      remember (match x with
+                | 0 => 1
+                | S n'' => Fib x + Fib n''
+                end). clear Heqn. rewrite Nat.sub_0_r. lia.
+    }
+    { init. unfold mainF, ccall. harg_tac. des; clarify.
+      iRefresh. iDestruct PRE. iPure A. des; clarify.
+      rewrite Any.upcast_downcast. ss. steps.
+      hexploit (SKINCL "fib"); ss; eauto. i. des.
+      rewrite H0. ss. steps.
+      astart 2.
+      eapply APC_step_clo with (fn:="knot") (args:=[Vptr blk 0]).
+      { try by
+            eapply Ord.eq_lt_lt;
+          [ symmetry; eapply OrdArith.add_from_nat
+          | eapply OrdArith.lt_from_nat; eapply Nat.lt_add_lt_sub_r;
+            eapply Nat.lt_succ_diag_r ]. }
+      { eauto. }
+      { ss. }
+      { eapply OrdArith.lt_from_nat; eapply Nat.lt_succ_diag_r. }
+      i. subst args'. iRefresh.
+      hcall_tac Fib (ord_pure 0) (@URA.unit Σ) (@URA.unit Σ) PRE; ss.
+      { splits; ss. iRefresh. iSplitR PRE; ss.
+        { red. red. esplits; eauto.
+          { eapply SKWF. eauto. }
+          { eapply FunStb_incl. des_ifs. }
+        }
+        { exists None. ss. }
+      }
+      des. clarify. iRefresh. iDestruct POST. iPure POST. des; clarify.
+      eapply Any.upcast_inj in POST. des; clarify.
+      steps. rewrite Any.upcast_downcast in _UNWRAPN. clarify.
+      ss. steps. rewrite POST0. steps.
+      eapply APC_step_clo with (fn0:=fn) (args:=[Vint 10]).
+      { try by
+            eapply Ord.eq_lt_lt;
+          [ symmetry; eapply OrdArith.add_from_nat
+          | eapply OrdArith.lt_from_nat; eapply Nat.lt_add_lt_sub_r;
+            eapply Nat.lt_succ_diag_r ]. }
+      { eauto. }
+      { ss. }
+      { eapply OrdArith.lt_from_nat; eapply Nat.lt_succ_diag_r. }
+      i. subst args'. iRefresh.
+
+      hcall_tac (Fib, 10) (ord_pure 21) (@URA.unit Σ) (@URA.unit Σ) A; ss.
+      { splits; ss. iRefresh. iSplitL A; ss. }
+      steps. des. clarify.
+      iRefresh. iDestruct POST. iPure A.
+      erewrite Any.upcast_downcast in _UNWRAPN. clarify.
+      eapply Any.upcast_inj in A. des; clarify.
+      astop. steps.
+      hret_tac (@URA.unit Σ) (@URA.unit Σ); ss.
+    }
+  Qed.
+
+End SIMMODSEM.
