examples/knot/KnotMain1.v
@@ -1,0 +1,76 @@
+Require Import Coqlib.
+Require Import Universe.
+Require Import STS.
+Require Import Behavior.
+Require Import ModSem.
+Require Import Skeleton.
+Require Import PCM.
+Require Import HoareDef.
+Require Import TODOYJ.
+Require Import Logic.
+Require Import KnotHeader.
+
+Generalizable Variables E R A B C X Y Σ.
+
+Set Implicit Arguments.
+
+
+
+Fixpoint Fib (n: nat): nat :=
+  match n with
+  | 0 => 1
+  | S n' =>
+    let r := Fib n' in
+    match n' with
+    | 0 => 1
+    | S n'' => r + Fib n''
+    end
+  end.
+
+Section MAIN.
+
+  Context `{Σ: GRA.t}.
+  Context `{@GRA.inG knotRA Σ}.
+
+  Variable RecStb: SkEnv.t -> list (gname * fspec).
+  Variable GlobalStb: SkEnv.t -> list (gname * fspec).
+
+  Section SKENV.
+    Variable skenv: SkEnv.t.
+
+    Definition fib_spec:    fspec := fun_gen RecStb skenv Fib.
+
+    Definition MainFunStb: list (gname * fspec) := [("fib", fib_spec)].
+
+    Definition main_spec:    fspec :=
+      mk_simple (X:=(nat -> nat))
+                (fun f => (
+                     (fun varg o =>
+                        Own (GRA.embed (knot_frag None)) ** ⌜o = ord_top⌝),
+                     (fun vret =>
+                        ⌜vret = (Vint (Z.of_nat (Fib 10)))↑⌝)
+                )).
+
+    Definition MainStb: list (gname * fspec) := [("fib", fib_spec); ("main", main_spec)].
+
+    Definition MainSbtb: list (gname * fspecbody) :=[("fib", mk_specbody fib_spec (fun _ => trigger (Choose _)));
+                                                    ("main", mk_specbody main_spec (fun _ => APC;; Ret (Vint (Z.of_nat (Fib 10)))))].
+
+    Definition SMainSem: SModSem.t := {|
+      SModSem.fnsems := MainSbtb;
+      SModSem.mn := "Main";
+      SModSem.initial_mr := ε;
+      SModSem.initial_st := tt↑;
+    |}
+    .
+  End SKENV.
+
+  Definition SMain: SMod.t := {|
+    SMod.get_modsem := SMainSem;
+    SMod.sk := [("fib", Sk.Gfun)];
+  |}
+  .
+
+  Definition Main: Mod.t := (SMod.to_tgt GlobalStb) SMain.
+
+End MAIN.
